UTP/ITree_DFP.thy
@@ -25,6 +25,58 @@ lemma dfp_seq [wp]: "dfp (P ;; Q) = (dfp P \<and> wlp P (dfp Q))\<^sub>e"
 lemma dfp_event_choice [wp]: "dfp (event_choice F) = (pdom(F) \<noteq> {} \<and> (\<forall> e\<in>pdom(F). dfp(F(\<guillemotleft>e\<guillemotright>)\<^sub>p)\<^sub>e))\<^sub>e"
   by (simp add: dfp_def event_choice_def deadlock_free_Vis SEXP_def)
 
+lemma dfp_event_block [wp]: "wb_prism c \<Longrightarrow> dfp (event_block c A (\<lambda> a. (P a, \<sigma> a))) = [\<lambda> s. \<exists> v\<in>A s. P v s]\<^sub>e"
+  by (simp add: dfp_def event_block_def deadlock_free_Vis_prism_fun SEXP_def) 
+
+(*
+lemma case_sum_prod_dist: "case_sum (\<lambda> x. (f\<^sub>1 x, f\<^sub>2 x)) (\<lambda> x. (g\<^sub>1 x, g\<^sub>2 x)) = (\<lambda> x. (case_sum f\<^sub>1 g\<^sub>1 x, case_sum f\<^sub>2 g\<^sub>2 x))"
+  by (simp add: fun_eq_iff sum.case_eq_if)
+
+lemma case_sum_Ret_dist: "(case a of Inl x \<Rightarrow> Ret (f x) | Inr y \<Rightarrow> Ret (g y)) = Ret (case a of Inl x \<Rightarrow> f x | Inr y \<Rightarrow> g y)"
+  by (simp add: sum.case_eq_if)
+  
+declare [[show_sorts]]
+
+lemma "c \<nabla> d \<Longrightarrow> event_block c A PB \<box> event_block d B QB = event_block (c +\<^sub>\<triangle> d) (A <+> B)\<^sub>e undefined"
+
+chantype chan =
+  Input :: nat
+  Output :: nat
+
+definition "Num = {0::nat..9}"
+
+find_theorems "(\<in>)" "(<+>)"
+
+lemma Inl_in_Sum_iff [simp]: "Inl x \<in> A <+> B \<longleftrightarrow> x \<in> A"
+  by fastforce
+
+lemma Inr_in_Sum_iff [simp]: "Inr y \<in> A <+> B \<longleftrightarrow> y \<in> B"
+  by fastforce
+
+term "Bex"
+
+lemma Bex_Sum_iff: "(\<exists>x\<in>A <+> B. P x) \<longleftrightarrow> (\<exists> x\<in>A. P (Inl x)) \<or> (\<exists> x\<in>B. P (Inr x))"
+  by (auto)
+
+lemma "deadlock_free (Vis (prism_fun Input Num (\<lambda> n. (True, Ret (buf @ [n]))) \<oplus> prism_fun Output Num (\<lambda> n. (length buf > 0 \<and> n = hd buf, Ret (tl buf)))))"
+  apply (simp add: prism_fun_combine case_sum_prod_dist case_sum_Ret_dist deadlock_free_Vis_prism_fun Bex_Sum_iff)
+  apply (auto simp add: Num_def)
+  done
+
+lemma "deadlock_free (Vis (prism_fun Output Num (\<lambda> n. (length buf > 0 \<and> n = hd buf, Ret (tl buf)))))"
+  apply (simp add: prism_fun_combine case_sum_prod_dist case_sum_Ret_dist deadlock_free_Vis_prism_fun Bex_Sum_iff)
+  nitpick
+  apply (rule deadlock_free_Vis_prism_fun)
+   apply (simp)
+  apply (rule_tac x="Inl 0" in exI)
+  apply simp
+
+lemma "deadlock_free (Vis (prism_fun Input Num (\<lambda> n. (True, Ret (buf @ [n])))))"
+  apply (rule deadlock_free_Vis_prism_fun)
+   apply (simp)
+  apply (auto simp add: Num_def)
+*)
+
 lemma deadlock_free_init_loop:
   assumes "\<sigma> establishes P" "C preserves P" "`P \<longrightarrow> dfp C`"
   shows "deadlock_free ((\<langle>\<sigma>\<rangle>\<^sub>a ;; loop C) s)"
